AVX2 alt2 implementation and proof

benchmarks/benchmark.c
@@ -1083,7 +1083,6 @@ void call_secp256k1_jmixadd_alt(void) repeat(secp256k1_jmixadd_alt(b1,b2,b3))
 
 void call_sha3_keccak_f1600(void) repeat(sha3_keccak_f1600(b0,b1))
 void call_sha3_keccak4_f1600(void) repeat(sha3_keccak4_f1600(b0,b1))
-void call_sha3_keccak4_f1600_alt(void) repeat(sha3_keccak4_f1600_alt(b0,b1,b3,b4))
 
 void call_sm2_montjadd(void) repeat(sm2_montjadd(b1,b2,b3))
 void call_sm2_montjadd_alt(void) repeat(sm2_montjadd_alt(b1,b2,b3))
@@ -1115,7 +1114,8 @@ void call_sha3_keccak_f1600_alt(void) {}
 void call_sha3_keccak_f1600_alt2(void) {}
 void call_sha3_keccak2_f1600(void) {}
 void call_sha3_keccak2_f1600_alt(void) {}
-void call_sha3_keccak4_f1600_alt2(void) {}
+void call_sha3_keccak4_f1600_alt(void) repeat(sha3_keccak4_f1600_alt2(b0,b1,b2,b3))
+void call_sha3_keccak4_f1600_alt2(void) repeat(sha3_keccak4_f1600_alt(b0,b1,b2,b3))
 
 #else
 
@@ -1140,6 +1140,7 @@ void call_sha3_keccak_f1600_alt(void) repeat(sha3_keccak_f1600_alt(b0,b1))
 void call_sha3_keccak_f1600_alt2(void) repeat(sha3_keccak_f1600_alt2(b0,b1))
 void call_sha3_keccak2_f1600(void) repeat(sha3_keccak2_f1600(b0,b1))
 void call_sha3_keccak2_f1600_alt(void) repeat(sha3_keccak2_f1600_alt(b0,b1))
+void call_sha3_keccak4_f1600_alt(void) repeat(sha3_keccak4_f1600_alt2(b0,b1))
 void call_sha3_keccak4_f1600_alt2(void) repeat(sha3_keccak4_f1600_alt2(b0,b1))
 
 void call_mlkem_frombytes(void) {}
@@ -1200,7 +1201,7 @@ int main(int argc, char *argv[])
   for (i = 0; i < 1000000; ++i) bignum_montmul(12,b0,b1,b2,b3);
 
   // Now the main tests
-
+#if 0
   timingtest(all,"bignum_add (4x4->4)",call_bignum_add__4_4);
   timingtest(all,"bignum_add (6x6->6)",call_bignum_add__6_6);
   timingtest(all,"bignum_add (32x32->32)",call_bignum_add__32_32);
@@ -1582,10 +1583,12 @@ int main(int argc, char *argv[])
   timingtest(arm,"sha3_keccak_f1600_alt2",call_sha3_keccak_f1600_alt2);
   timingtest(sha3,"sha3_keccak2_f1600",call_sha3_keccak2_f1600);
   timingtest(sha3,"sha3_keccak2_f1600_alt",call_sha3_keccak2_f1600_alt);
+  #endif
   timingtest(all,"sha3_keccak_f1600",call_sha3_keccak_f1600);
   timingtest(all,"sha3_keccak4_f1600",call_sha3_keccak4_f1600);
   timingtest(all,"sha3_keccak4_f1600_alt",call_sha3_keccak4_f1600_alt);
-  timingtest(sha3,"sha3_keccak4_f1600_alt2",call_sha3_keccak4_f1600_alt2);
+  timingtest(all,"sha3_keccak4_f1600_alt2",call_sha3_keccak4_f1600_alt2);
+  #if 0
   timingtest(bmi,"sm2_montjadd",call_sm2_montjadd);
   timingtest(all,"sm2_montjadd_alt",call_sm2_montjadd_alt);
   timingtest(bmi,"sm2_montjdouble",call_sm2_montjdouble);
@@ -1603,7 +1606,7 @@ int main(int argc, char *argv[])
   timingtest(all,"word_negmodinv",call_word_negmodinv);
   timingtest(all,"word_popcount",call_word_popcount);
   timingtest(all,"word_recip",call_word_recip);
-
+#endif
   // Summarize performance in arithmetic and geometric means
 
   arithmean /= (double) tests;
