tests/test.c
@@ -14300,9 +14300,6 @@ int test_sha3_keccak4_f1600_alt(void)
 
 int test_sha3_keccak4_f1600_alt2(void)
 {
-#ifdef __x86_64__
-  return 1;
-#else
   uint64_t t, i;
   uint64_t a[100], b[100], c[100];
   printf("Testing sha3_keccak4_f1600_alt2 with %d cases\n",tests);
@@ -14314,7 +14311,11 @@ int test_sha3_keccak4_f1600_alt2(void)
      reference_keccak_f1600(b+25,a+25);
      reference_keccak_f1600(b+50,a+50);
      reference_keccak_f1600(b+75,a+75);
-     sha3_keccak4_f1600_alt2(c,keccak_RC);
+      #ifdef __x86_64__
+       sha3_keccak4_f1600_alt2(c,keccak_RC, rho8, rho56);
+     #else
+       sha3_keccak4_f1600_alt2(c,keccak_RC);
+     #endif
      for (i = 0; i < 100; ++i)
       { if (b[i] != c[i])
          { printf("Error in keccak4_f1600 batch = %"PRIu64", element i = %"PRIu64"; "
@@ -14334,7 +14335,6 @@ int test_sha3_keccak4_f1600_alt2(void)
    }
   printf("All OK\n");
   return 0;
-#endif
 }
 
 int test_sm2_montjadd(void)
@@ -15461,7 +15461,7 @@ int main(int argc, char *argv[])
    }
 
   if (tests == 0) tests = TESTS;
-
+#if 0
   functionaltest(all,"bignum_add",test_bignum_add);
   functionaltest(all,"bignum_add_p25519",test_bignum_add_p25519);
   functionaltest(all,"bignum_add_p256",test_bignum_add_p256);
@@ -15788,7 +15788,10 @@ int main(int argc, char *argv[])
   functionaltest(all,"secp256k1_jmixadd_alt",test_secp256k1_jmixadd_alt);
   functionaltest(all,"sha3_keccak_f1600",test_sha3_keccak_f1600);
   functionaltest(all,"sha3_keccak4_f1600",test_sha3_keccak4_f1600);
+  #endif
   functionaltest(all,"sha3_keccak4_f1600_alt",test_sha3_keccak4_f1600_alt);
+  functionaltest(all,"sha3_keccak4_f1600_alt2",test_sha3_keccak4_f1600_alt2);
+  #if 0
   functionaltest(bmi,"sm2_montjadd",test_sm2_montjadd);
   functionaltest(all,"sm2_montjadd_alt",test_sm2_montjadd_alt);
   functionaltest(bmi,"sm2_montjdouble",test_sm2_montjdouble);
@@ -15816,7 +15819,6 @@ int main(int argc, char *argv[])
     functionaltest(arm,"sha3_keccak_f1600_alt2",test_sha3_keccak_f1600_alt2);
     functionaltest(sha3,"sha3_keccak2_f1600",test_sha3_keccak2_f1600);
     functionaltest(sha3,"sha3_keccak2_f1600_alt",test_sha3_keccak2_f1600_alt);
-    functionaltest(sha3,"sha3_keccak4_f1600_alt2",test_sha3_keccak4_f1600_alt2);
 
   }
 
@@ -15834,7 +15836,7 @@ int main(int argc, char *argv[])
   functionaltest(all,"curve25519_x25519base_byte_alt (TweetNaCl)",test_curve25519_x25519base_byte_alt_tweetnacl);
   functionaltest(bmi,"edwards25519_scalarmulbase (TweetNaCl)",test_edwards25519_scalarmulbase_tweetnacl);
   functionaltest(all,"edwards25519_scalarmulbase_alt (TweetNaCl)",test_edwards25519_scalarmulbase_alt_tweetnacl);
-
+#endif
   if (successes == tested)
    { printf("All %d tests run, all passed\n",successes);
      return 0;
